{-# OPTIONS --safe #-} -- --without-K #-}

open import Function using (_âˆ˜_; id)
open import Data.Empty using (âŠ¥-elim)
open import Relation.Binary.PropositionalEquality using (_â‰¡_; _â‰¢_; refl; trans; sym; cong; congâ‚‚)
open Relation.Binary.PropositionalEquality.â‰¡-Reasoning
open import Data.Product using (Î£-syntax; _,_)
open import Data.Unit using (tt)
open import Relation.Nullary using (yes; no)

import Data.Nat as â„•
import Data.Nat.Properties as â„•â‚š
import Data.Fin as Fin
import Data.Fin.Properties as Finâ‚š

open â„• using (â„•; zero; suc)
open Fin using (Fin; zero; suc)

open import PiCalculus.Syntax
open Scoped
open import PiCalculus.Semantics

module PiCalculus.Semantics.Properties where
private
  variable
    n m l : â„•
    i j : Fin n
    P : Scoped n


lift-lower : (i : Fin (suc n)) (P : Scoped (suc n)) (uP : Unused i P)
           â†’ |> suc (lower i P uP) â‰¡ P
lift-lower {n = zero} zero ğŸ˜ uP = refl
lift-lower {n = zero} zero (Î½ P) uP rewrite lift-lower (suc zero) P uP = {!!}
lift-lower {n = zero} zero (P âˆ¥ Pâ‚) uP = {!!}
lift-lower {n = zero} zero (x â¦…â¦† P) uP = {!!}
lift-lower {n = zero} zero (x âŸ¨ xâ‚ âŸ© P) uP = {!!}
lift-lower {n = suc n} i ğŸ˜ uP = refl
lift-lower {n = suc n} i (Î½ P) uP
  rewrite lift-lower (suc i) P uP = {!refl!}
lift-lower {n = suc n} i (P âˆ¥ Q) (uP , uQ)
  rewrite lift-lower i P uP
  | lift-lower i Q uQ = {!!}
lift-lower {n = suc n} i (x â¦…â¦† P) (iâ‰¢x , uP)
  rewrite lift-lower (suc i) P uP
  | Finâ‚š.punchIn-punchOut iâ‰¢x = {!!}
lift-lower {n = suc n} i (x âŸ¨ y âŸ© P) (iâ‰¢x , iâ‰¢y , uP)
  rewrite lift-lower i P uP
  | Finâ‚š.punchIn-punchOut iâ‰¢x
  | Finâ‚š.punchIn-punchOut iâ‰¢y = {!!}

exchangeFin-exchangeFin : âˆ€ (i : Fin n) (x : Fin (suc n)) â†’ exchangeFin i (exchangeFin i x) â‰¡ x
exchangeFin-exchangeFin zero zero = refl
exchangeFin-exchangeFin zero (suc zero) = refl
exchangeFin-exchangeFin zero (suc (suc x)) = refl
exchangeFin-exchangeFin (suc i) zero = refl
exchangeFin-exchangeFin (suc i) (suc x) = cong suc (exchangeFin-exchangeFin i x)

suc-|>-cong : (g f : Fin n â†’ Fin m) â†’ (âˆ€ x â†’ f x â‰¡ g x) â†’ (âˆ€ x â†’ suc-|> f x â‰¡ suc-|> g x)
suc-|>-cong g f eq zero = refl
suc-|>-cong g f eq (suc x) = cong suc (eq x)

suc-|>-comp : (g : Fin n â†’ Fin m) (f : Fin m â†’ Fin l) (x : Fin (suc n)) â†’ suc-|> (f âˆ˜ g) x â‰¡ (suc-|> f âˆ˜ suc-|> g) x
suc-|>-comp g f zero = refl
suc-|>-comp g f (suc x) = refl

suc-|>-id : (x : Fin (suc n)) â†’ (suc-|> id) x â‰¡ x
suc-|>-id zero = refl
suc-|>-id (suc x) = refl

|>-ext : (g f : Fin n â†’ Fin m) â†’ (âˆ€ x â†’ f x â‰¡ g x) â†’ (âˆ€ P â†’ |> f P â‰¡ |> g P)
|>-ext g f eq ğŸ˜ = refl
|>-ext g f eq (Î½ P) = cong (Î» â— â†’ Î½ â—) (|>-ext (suc-|> g) (suc-|> f) (suc-|>-cong g f eq) P)
|>-ext g f eq (P âˆ¥ Q) = congâ‚‚ _âˆ¥_ (|>-ext g f eq P) (|>-ext g f eq Q)
|>-ext g f eq (x â¦…â¦† P) rewrite eq x = cong (_ â¦…â¦†_) (|>-ext (suc-|> g) (suc-|> f) (suc-|>-cong g f eq) P)
|>-ext g f eq (x âŸ¨ y âŸ© P) rewrite eq x | eq y = cong (_ âŸ¨ _ âŸ©_) (|>-ext g f eq P)

|>-id : (P : Scoped n) â†’ |> id P â‰¡ P
|>-id ğŸ˜ = refl
|>-id (Î½ P) rewrite |>-ext _ _ suc-|>-id P = cong (Î» â— â†’ Î½ â—) (|>-id P)
|>-id (P âˆ¥ Q) = congâ‚‚ _âˆ¥_ (|>-id P) (|>-id Q)
|>-id (x â¦…â¦† P) rewrite |>-ext _ _ suc-|>-id P = cong (_ â¦…â¦†_) (|>-id P)
|>-id (x âŸ¨ y âŸ© P) = cong (_ âŸ¨ _ âŸ©_) (|>-id P)

|>-comp : (g : Fin n â†’ Fin m) (f : Fin m â†’ Fin l) (P : Scoped n) â†’ |> f (|> g P) â‰¡ |> (f âˆ˜ g) P
|>-comp g f ğŸ˜ = refl
|>-comp g f (Î½ P)
  rewrite |>-ext _ _ (suc-|>-comp g f) P = cong (Î» â— â†’ Î½ â—) (|>-comp _ _ P)
|>-comp g f (P âˆ¥ Q) = congâ‚‚ _âˆ¥_ (|>-comp g f P) (|>-comp g f Q)
|>-comp g f (x â¦…â¦† P)
  rewrite |>-ext _ _ (suc-|>-comp g f) P = cong (_ â¦…â¦†_) (|>-comp _ _ P)
|>-comp g f (x âŸ¨ y âŸ© P) = cong (_ âŸ¨ _ âŸ©_) (|>-comp _ _ P)

exchange-exchange : âˆ€ (i : Fin n) (P : Scoped (suc n)) â†’ |> (exchangeFin  i) (|> (exchangeFin i) P) â‰¡ P
exchange-exchange i P
  rewrite |>-comp (exchangeFin i) (exchangeFin i) P
  | |>-ext _ _ (exchangeFin-exchangeFin i) P = |>-id P
